Rename permutation definitions

Permutation.v
@@ -1,113 +1,86 @@
 Load ListCost.
 
-Inductive is_permutation_alt {A} : list A -> list A -> Prop :=
-  | is_permutation_alt_empty : is_permutation_alt [] []
-  | is_permutation_alt_insert a l1 l2 l3 :
-    is_permutation_alt (l1 ++ l2) l3 ->
-    is_permutation_alt (l1 ++ a :: l2) (a :: l3).
+Inductive permutation {A} : list A -> list A -> Prop :=
+  | permutation_nil : permutation [] []
+  | permutation_insert a l1 l2 l3 :
+    permutation (l1 ++ l2) l3 ->
+    permutation (l1 ++ a :: l2) (a :: l3).
 
-Inductive is_permutation {A} : list A -> list A -> Prop :=
-  | is_permutation_empty : is_permutation [] []
-  | is_permutation_add a l1 l2 : is_permutation l1 l2 -> is_permutation (a :: l1) (a :: l2)
-  | is_permutation_swap a b l : is_permutation (b :: a :: l) (a :: b :: l)
-  | is_permutation_trans l1 l2 l3 : is_permutation l1 l2 -> is_permutation l2 l3 -> is_permutation l1 l3.
+Inductive permutation_small {A} : list A -> list A -> Prop :=
+  | permutation_small_empty : permutation_small [] []
+  | permutation_small_cons a l1 l2 : permutation_small l1 l2 -> permutation_small (a :: l1) (a :: l2)
+  | permutation_small_swap a b l : permutation_small (b :: a :: l) (a :: b :: l)
+  | permutation_small_trans l1 l2 l3 :
+    permutation_small l1 l2 ->
+    permutation_small l2 l3 ->
+    permutation_small l1 l3.
 
 Section Example.
 
-Theorem is_permutation_example : is_permutation [5; 3; 1; 2; 4] [1; 2; 3; 4; 5].
+Theorem permutation_example : permutation [5; 3; 1; 2; 4] [1; 2; 3; 4; 5].
 Proof.
-  apply is_permutation_trans with [5; 1; 3; 2; 4].
-  apply is_permutation_add.
-  apply is_permutation_swap.
-  apply is_permutation_trans with [1; 5; 3; 2; 4].
-  apply is_permutation_swap.
-  apply is_permutation_add.
-  apply is_permutation_trans with [5; 2; 3; 4].
-  apply is_permutation_add.
-  apply is_permutation_swap.
-  apply is_permutation_trans with [2; 5; 3; 4].
-  apply is_permutation_swap.
-  apply is_permutation_add.
-  apply is_permutation_trans with [3; 5; 4].
-  apply is_permutation_swap.
-  apply is_permutation_add.
-  apply is_permutation_swap.
+  replace [5; 3; 1; 2; 4] with ([5; 3] ++ 1 :: [2; 4]) by auto; apply permutation_insert; simpl.
+  replace [5; 3; 2; 4] with ([5; 3] ++ 2 :: [4]) by auto; apply permutation_insert; simpl.
+  replace [5; 3; 4] with ([5] ++ 3 :: [4]) by auto; apply permutation_insert; simpl.
+  replace [5; 4] with ([5] ++ 4 :: []) by auto; apply permutation_insert; simpl.
+  replace [5] with ([] ++ 5 :: []) by auto; apply permutation_insert; simpl.
+  apply permutation_nil.
+Qed.
+
+Theorem permutation_example_move : permutation [5; 3; 1; 2; 4] [3; 1; 2; 4; 5].
+Proof.
+  replace [5; 3; 1; 2; 4] with ([5] ++ 3 :: [1; 2; 4]) by auto; apply permutation_insert; simpl.
+  replace [5; 1; 2; 4] with ([5] ++ 1 :: [2; 4]) by auto; apply permutation_insert; simpl.
+  replace [5; 2; 4] with ([5] ++ 2 :: [4]) by auto; apply permutation_insert; simpl.
+  replace [5; 4] with ([5] ++ 4 :: []) by auto; apply permutation_insert; simpl.
+  replace [5] with ([] ++ 5 :: []) by auto; apply permutation_insert; simpl.
+  apply permutation_nil.
+Qed.
+
+Theorem permutation_example_sym : permutation [1; 2; 3; 4; 5] [5; 3; 1; 2; 4].
+Proof.
+  replace [1; 2; 3; 4; 5] with ([1; 2; 3; 4] ++ 5 :: []) by auto; apply permutation_insert; simpl.
+  replace [1; 2; 3; 4] with ([1; 2] ++ 3 :: [4]) by auto; apply permutation_insert; simpl.
+  replace [1; 2; 4] with ([] ++ 1 :: [2; 4]) by auto; apply permutation_insert; simpl.
+  replace [2; 4] with ([] ++ 2 :: [4]) by auto; apply permutation_insert; simpl.
+  replace [4] with ([] ++ 4 :: []) by auto; apply permutation_insert; simpl.
+  apply permutation_nil.
+Qed.
+
+Theorem permutation_small_example : permutation_small [5; 3; 1; 2; 4] [1; 2; 3; 4; 5].
+Proof.
+  apply permutation_small_trans with [5; 1; 3; 2; 4].
+  apply permutation_small_cons.
+  apply permutation_small_swap.
+  apply permutation_small_trans with [1; 5; 3; 2; 4].
+  apply permutation_small_swap.
+  apply permutation_small_cons.
+  apply permutation_small_trans with [5; 2; 3; 4].
+  apply permutation_small_cons.
+  apply permutation_small_swap.
+  apply permutation_small_trans with [2; 5; 3; 4].
+  apply permutation_small_swap.
+  apply permutation_small_cons.
+  apply permutation_small_trans with [3; 5; 4].
+  apply permutation_small_swap.
+  apply permutation_small_cons.
+  apply permutation_small_swap.
 Qed.
 
 End Example.
 
-Theorem is_permutation_refl : forall {A} (l : list A), is_permutation l l.
+Theorem permutation_small_refl : forall {A} (l : list A), permutation_small l l.
 Proof.
   induction l.
-  - apply is_permutation_empty.
-  - apply is_permutation_add. auto.
+  - apply permutation_small_empty.
+  - apply permutation_small_cons. auto.
 Qed.
 
-Theorem is_permutation_sym : forall {A} (l1 l2 : list A), is_permutation l1 l2 -> is_permutation l2 l1.
-Proof.
-  intros ? ? ? ?. induction H.
-  - apply is_permutation_empty.
-  - apply is_permutation_add. auto.
-  - apply is_permutation_swap.
-  - apply is_permutation_trans with l2; auto.
-Qed.
-
-Section Unused.
-
-Fixpoint rev {A} (l : list A) :=
-  match l with
-  | [] => []
-  | x :: l' => rev l' ++ [x]
-  end.
-
-Theorem list_empty_or_not_empty : forall {A} (l : list A), {l = []} + {l <> []}.
-Proof.
-  intros ? l. destruct l.
-  - left. auto.
-  - right. discriminate.
-Qed.
-
-End Unused.
-
-Section Example.
-
-Theorem is_permutation_alt_example : is_permutation_alt [5; 3; 1; 2; 4] [1; 2; 3; 4; 5].
-Proof.
-  replace [5; 3; 1; 2; 4] with ([5; 3] ++ 1 :: [2; 4]) by auto; apply is_permutation_alt_insert; simpl.
-  replace [5; 3; 2; 4] with ([5; 3] ++ 2 :: [4]) by auto; apply is_permutation_alt_insert; simpl.
-  replace [5; 3; 4] with ([5] ++ 3 :: [4]) by auto; apply is_permutation_alt_insert; simpl.
-  replace [5; 4] with ([5] ++ 4 :: []) by auto; apply is_permutation_alt_insert; simpl.
-  replace [5] with ([] ++ 5 :: []) by auto; apply is_permutation_alt_insert; simpl.
-  apply is_permutation_alt_empty.
-Qed.
-
-Theorem is_permutation_alt_example_move : is_permutation_alt [5; 3; 1; 2; 4] [3; 1; 2; 4; 5].
-Proof.
-  replace [5; 3; 1; 2; 4] with ([5] ++ 3 :: [1; 2; 4]) by auto; apply is_permutation_alt_insert; simpl.
-  replace [5; 1; 2; 4] with ([5] ++ 1 :: [2; 4]) by auto; apply is_permutation_alt_insert; simpl.
-  replace [5; 2; 4] with ([5] ++ 2 :: [4]) by auto; apply is_permutation_alt_insert; simpl.
-  replace [5; 4] with ([5] ++ 4 :: []) by auto; apply is_permutation_alt_insert; simpl.
-  replace [5] with ([] ++ 5 :: []) by auto; apply is_permutation_alt_insert; simpl.
-  apply is_permutation_alt_empty.
-Qed.
-
-Theorem is_permutation_alt_example_sym : is_permutation_alt [1; 2; 3; 4; 5] [5; 3; 1; 2; 4].
-Proof.
-  replace [1; 2; 3; 4; 5] with ([1; 2; 3; 4] ++ 5 :: []) by auto; apply is_permutation_alt_insert; simpl.
-  replace [1; 2; 3; 4] with ([1; 2] ++ 3 :: [4]) by auto; apply is_permutation_alt_insert; simpl.
-  replace [1; 2; 4] with ([] ++ 1 :: [2; 4]) by auto; apply is_permutation_alt_insert; simpl.
-  replace [2; 4] with ([] ++ 2 :: [4]) by auto; apply is_permutation_alt_insert; simpl.
-  replace [4] with ([] ++ 4 :: []) by auto; apply is_permutation_alt_insert; simpl.
-  apply is_permutation_alt_empty.
-Qed.
-
-End Example.
-
-Theorem is_permutation_alt_refl : forall {A} (l : list A), is_permutation_alt l l.
+Theorem permutation_refl : forall {A} (l : list A), permutation l l.
 Proof.
   induction l.
-  - apply is_permutation_alt_empty.
-  - replace (a :: l) with ([] ++ a :: l) by auto. apply is_permutation_alt_insert. auto.
+  - apply permutation_nil.
+  - replace (a :: l) with ([] ++ a :: l) by auto. apply permutation_insert. auto.
 Qed.
 
 Lemma app_insert_split :
@@ -128,158 +101,170 @@ Proof.
       * right. exists l5. auto.
 Qed.
 
-Lemma permutation_alt_split:
+Lemma permutation_split:
   forall {A} a (l1 l2 l3 : list A),
-  is_permutation_alt l1 (l2 ++ a :: l3) ->
-  exists l4 l5, l1 = l4 ++ a :: l5 /\ is_permutation_alt (l4 ++ l5) (l2 ++ l3).
+  permutation l1 (l2 ++ a :: l3) ->
+  exists l4 l5, l1 = l4 ++ a :: l5 /\ permutation (l4 ++ l5) (l2 ++ l3).
 Proof.
   intros ? a l1 l2 l3 ?. remember (l2 ++ a :: l3) as l4. generalize dependent l2. induction H; intros l2' Heql4.
   - destruct l2'; discriminate.
   - rename a0 into b. destruct l2'.
     + injection Heql4 as <- ->. exists l1, l2. auto.
     + injection Heql4 as <- ->.
-      specialize (IHis_permutation_alt l2' eq_refl).  destruct IHis_permutation_alt as (l9 & l10 & ? & ?).
+      specialize (IHpermutation l2' eq_refl).  destruct IHpermutation as (l9 & l10 & ? & ?).
       apply app_insert_split in H0. destruct H0 as [(l6 & -> & ->) | (l6 & -> & ->)].
       * rewrite app_assoc in H1. exists (l1 ++ b :: l6), l10. simpl. split.
         -- rewrite app_assoc. auto.
-        -- rewrite app_assoc. simpl. apply is_permutation_alt_insert. auto.
+        -- rewrite app_assoc. simpl. apply permutation_insert. auto.
       * rewrite app_assoc in H. exists l9, (l6 ++ b :: l2). simpl. split.
         -- rewrite app_assoc. auto.
-        -- rewrite <- app_assoc. apply is_permutation_alt_insert. rewrite app_assoc. auto.
+        -- rewrite <- app_assoc. apply permutation_insert. rewrite app_assoc. auto.
 Qed.
 
-Lemma is_permutation_alt_move :
+Lemma permutation_move :
   forall {A} a (l1 l2 l3 : list A),
-  is_permutation_alt l1 (l2 ++ a :: l3) ->
-  is_permutation_alt l1 (a :: l2 ++ l3).
+  permutation l1 (l2 ++ a :: l3) ->
+  permutation l1 (a :: l2 ++ l3).
 Proof.
   intros A a l1 l2 l3 ?.
-  apply permutation_alt_split in H. destruct H as (l4 & l5 & -> & ?).
-  apply is_permutation_alt_insert. auto.
+  apply permutation_split in H. destruct H as (l4 & l5 & -> & ?).
+  apply permutation_insert. auto.
 Qed.
 
-Theorem is_permutation_alt_trans :
+Theorem permutation_trans :
   forall {A} (l1 l2 l3 : list A),
-  is_permutation_alt l1 l2 ->
-  is_permutation_alt l2 l3 ->
-  is_permutation_alt l1 l3.
+  permutation l1 l2 ->
+  permutation l2 l3 ->
+  permutation l1 l3.
 Proof.
   intros ? l1 l2 l3 ? ?.
   generalize dependent l2. generalize dependent l1. induction l3; intros l1 l2 H1 H2.
   - inversion H2. subst l2. auto.
   - inversion H2. subst a0 l2 l5. clear H2.
-    apply is_permutation_alt_move in H1.
-    inversion H1. subst a0 l1 l6. apply is_permutation_alt_insert. apply IHl3 with (l0 ++ l4); auto.
+    apply permutation_move in H1.
+    inversion H1. subst a0 l1 l6. apply permutation_insert. apply IHl3 with (l0 ++ l4); auto.
 Qed.
 
-Theorem is_permutation_alt_sym :
+Theorem permutation_sym :
   forall {A} (l1 l2 : list A),
-  is_permutation_alt l1 l2 ->
-  is_permutation_alt l2 l1.
+  permutation l1 l2 ->
+  permutation l2 l1.
 Proof.
   intros ? l1 l2 ?. generalize dependent l1. induction l2; intros l1 ?.
-  - inversion H. apply is_permutation_alt_empty.
+  - inversion H. apply permutation_nil.
   - inversion H. subst a0 l1 l4. clear H. apply IHl2 in H2. clear IHl2.
     generalize dependent l3. generalize dependent l2. induction l0; intros l2 l3 ?.
     + simpl. simpl in H2. replace (a :: l2) with ([] ++ a :: l2) by auto.
-      apply is_permutation_alt_insert. auto.
+      apply permutation_insert. auto.
     + rename a0 into b. simpl in H2. inversion H2. subst a0 l2 l5. simpl.
       replace (a :: l1 ++ b :: l4) with ((a :: l1) ++ b :: l4) by auto.
-      apply is_permutation_alt_insert. simpl. auto.
+      apply permutation_insert. simpl. auto.
 Qed.
 
-Theorem is_permutation_alt_is_permutation :
+Theorem permutation_cons :
+  forall {A} a (l1 l2 : list A),
+  permutation l1 l2 ->
+  permutation (a :: l1) (a :: l2).
+Proof.
+  intros ? ? ? ? ?. replace (a :: l1) with ([] ++ a :: l1) by auto. apply permutation_insert. auto.
+Qed.
+
+Theorem permutation_swap :
+  forall {A} a b (l1 l2 : list A),
+  permutation l1 l2 ->
+  permutation (b :: a :: l1) (a :: b :: l2).
+Proof.
+  intros ? ? ? ? ? ?.
+  replace (b :: a :: l1) with ([b] ++ a :: l1) by auto. apply permutation_insert.
+  apply permutation_cons. auto.
+Qed.
+
+Theorem permutation_small_permutation :
   forall {A} (l1 l2 : list A),
-  is_permutation_alt l1 l2 <-> is_permutation l1 l2.
+  permutation_small l1 l2 <-> permutation l1 l2.
 Proof.
   intros ? l1 l2. split.
   - intros ?. induction H.
-    + apply is_permutation_empty.
-    + apply is_permutation_trans with (a :: l1 ++ l2).
-      * clear H IHis_permutation_alt l3. induction l1.
-        -- simpl. apply is_permutation_refl.
-        -- rename a0 into b. simpl. apply is_permutation_trans with (b :: a :: l1 ++ l2).
-           ++ apply is_permutation_add. auto.
-           ++ apply is_permutation_swap.
-      * apply is_permutation_add. auto.
-  - intros ?. induction H.
-    + apply is_permutation_alt_empty.
-    + replace (a :: l1) with ([] ++ a :: l1) by auto. apply is_permutation_alt_insert; auto.
-    + cut (is_permutation_alt (b :: [a] ++ l) (a :: [b] ++ l)).
+    + apply permutation_nil.
+    + replace (a :: l1) with ([] ++ a :: l1) by auto. apply permutation_insert; auto.
+    + cut (permutation (b :: [a] ++ l) (a :: [b] ++ l)).
       * auto.
-      * apply is_permutation_alt_move. apply is_permutation_alt_refl.
-    + clear H H0. apply is_permutation_alt_trans with l2; auto.
+      * apply permutation_move. apply permutation_refl.
+    + clear H H0. apply permutation_trans with l2; auto.
+  - intros ?. induction H.
+    + apply permutation_small_empty.
+    + apply permutation_small_trans with (a :: l1 ++ l2).
+      * clear H IHpermutation l3. induction l1.
+        -- simpl. apply permutation_small_refl.
+        -- rename a0 into b. simpl. apply permutation_small_trans with (b :: a :: l1 ++ l2).
+           ++ apply permutation_small_cons. auto.
+           ++ apply permutation_small_swap.
+      * apply permutation_small_cons. auto.
 Qed.
 
-Theorem permutation_length : forall {A} (l1 l2 : list A), is_permutation l1 l2 -> length l2 = length l1.
+Theorem permutation_length : forall {A} (l1 l2 : list A), permutation l1 l2 -> length l2 = length l1.
 Proof.
-  setoid_rewrite <- is_permutation_alt_is_permutation.
   intros ? ? ? ?. induction H.
   - auto.
-  - rewrite length_app. rewrite length_app in IHis_permutation_alt. simpl. lia.
+  - rewrite length_app. rewrite length_app in IHpermutation. simpl. lia.
 Qed.
 
 Theorem list_forall_permutation :
   forall {A} f (l1 l2 : list A),
-  is_permutation_alt l1 l2 ->
+  permutation l1 l2 ->
   list_forall f l1 -> list_forall f l2.
 Proof.
   intros ? ? ? ? ?. induction H; intros ?.
   - auto.
   - simpl. apply list_forall_app in H0. simpl in H0.
-    rewrite list_forall_app in IHis_permutation_alt. intuition auto.
+    rewrite list_forall_app in IHpermutation. intuition auto.
 Qed.
 
 Theorem permutation_same_head_inversion :
   forall {A} a (l1 l2 : list A),
-  is_permutation (a :: l1) (a :: l2) ->
-  is_permutation l1 l2.
+  permutation (a :: l1) (a :: l2) ->
+  permutation l1 l2.
 Proof.
-  setoid_rewrite <- is_permutation_alt_is_permutation.
   intros ? ? ? ? ?. inversion H. subst a0 l4. destruct l0.
   - injection H0 as ->. auto.
-  - injection H0 as -> <-. apply is_permutation_alt_trans with (a  :: l0 ++ l3).
-    + apply is_permutation_alt_move. apply is_permutation_alt_refl.
+  - injection H0 as -> <-. apply permutation_trans with (a  :: l0 ++ l3).
+    + apply permutation_move. apply permutation_refl.
     + auto.
 Qed.
 
 Theorem app_permutation_inversion :
   forall {A} (l1 l2 l3 l4 : list A),
-  is_permutation (l1 ++ l3) (l2 ++ l4) ->
-  is_permutation l1 l2 ->
-  is_permutation l3 l4.
+  permutation (l1 ++ l3) (l2 ++ l4) ->
+  permutation l1 l2 ->
+  permutation l3 l4.
 Proof.
-  setoid_rewrite <- is_permutation_alt_is_permutation.
   intros ? ? ? ? ? ? ?. generalize dependent l4. generalize dependent l3. induction H0; intros l3_ l4_ ?.
   - auto.
   - rewrite app_assoc in H. simpl in H.
-    apply is_permutation_alt_sym in H. apply is_permutation_alt_move in H. apply is_permutation_alt_sym in H.
-    apply is_permutation_alt_is_permutation in H. apply permutation_same_head_inversion in H.
-    apply is_permutation_alt_is_permutation in H. apply IHis_permutation_alt. rewrite app_assoc. auto.
+    apply permutation_sym in H. apply permutation_move in H. apply permutation_sym in H.
+    apply permutation_same_head_inversion in H. apply IHpermutation. rewrite app_assoc. auto.
 Qed.
 
-Theorem permutation_empty_inversion :
+Theorem permutation_nil_inversion :
   forall {A} (l : list A),
-  is_permutation l [] ->
+  permutation l [] ->
   l = [].
 Proof.
-  setoid_rewrite <- is_permutation_alt_is_permutation.
   intros ? ? ?. inversion H. auto.
 Qed.
 
 Theorem permutation_single_inversion :
   forall {A} a (l : list A),
-  is_permutation l [a] ->
+  permutation l [a] ->
   l = [a].
 Proof.
-  setoid_rewrite <- is_permutation_alt_is_permutation.
-  intros ? ? ? ?. inversion H. subst a0 l3. rewrite is_permutation_alt_is_permutation in H2.
-  apply permutation_empty_inversion in H2. apply app_empty_inversion in H2. destruct H2 as (-> & ->). auto.
+  intros ? ? ? ?. inversion H. subst a0 l3. apply permutation_nil_inversion in H2.
+  apply app_nil_inversion in H2. destruct H2 as (-> & ->). auto.
 Qed.
 
 Theorem permutation_single_inversion' :
   forall {A} (a b : A),
-  is_permutation [a] [b] ->
+  permutation [a] [b] ->
   a = b.
 Proof.
   intros ? ? ? ?. apply permutation_single_inversion in H. injection H as ->. auto.
@@ -287,14 +272,12 @@ Qed.
 
 Theorem permutation_cons_inversion :
   forall {A} a b (l1 l2 : list A),
-  is_permutation (a :: l1) (b :: l2) ->
+  permutation (a :: l1) (b :: l2) ->
   a = b \/ list_in a l2 /\ list_in b l1.
 Proof.
-  setoid_rewrite <- is_permutation_alt_is_permutation.
   intros ? ? ? ? ? ?. inversion H. subst a0 l4. destruct l0.
   - injection H0 as -> ->. left. auto.
   - injection H0 as -> <-. right. split.
-    + apply is_permutation_alt_sym in H2. inversion H2. subst a0 l5. apply list_in_insert.
+    + apply permutation_sym in H2. inversion H2. subst a0 l5. apply list_in_insert.
     + apply list_in_insert.
 Qed.
-
